

Limit Techniques

Type of limit	$x \rightarrow$	Technique
Limits to infinity	$\pm\infty$	Divide by highest power in denominator
Fraction of polynomials	Number	Factor and cancel
$\sqrt{x+\dots}-n$	Number	Multiply by $\frac{\sqrt{x+\dots}+n}{\sqrt{x+\dots}+n}$
$\frac{\sin nx}{x}$	0	This is always equal to n
$\frac{\sin}{\sin}$	0	Multiply by $\frac{x}{x}$
$\tan x$	Number	Express tan in terms of sin and cos
$1 - \cos$ or $1 - \sin$	$0, \frac{\pi}{2}, \pi, 2\pi$	Multiply by conjugate and use $\cos^2 + \sin^2 = 1$

Examples:

0.1 Limits to Infinity

We need to remember 3 basic types of limits here:

$$\lim_{x \rightarrow \infty} \frac{1}{x^n} = 0$$

$$\lim_{x \rightarrow -\infty} \frac{1}{x^n} = 0$$
(1)

when $n > 0$.

$$\lim_{x \rightarrow \infty} x^{\text{EVEN}} = \infty$$

$$\lim_{x \rightarrow -\infty} x^{\text{EVEN}} = \infty$$
(2)

$$\begin{aligned}\lim_{x \rightarrow \infty} x^{\text{ODD}} &= \infty \\ \lim_{x \rightarrow -\infty} x^{\text{ODD}} &= -\infty\end{aligned}\tag{3}$$

Example 0.1.1: •

Find $\lim_{x \rightarrow \infty} \frac{x^2 + 3x - 1}{x^5 + 2}$

The highest power is in the denominator, so this should be zero. If we divide by the highest power in the denominator (x^5) we get

$$\lim_{x \rightarrow \infty} \frac{\frac{1}{x^3} + 3\frac{1}{x^4} - \frac{1}{x^5}}{1 + 2\frac{1}{x^5}} = \frac{0 + 0 + 0}{1 + 0} = 0\tag{4}$$

Example 0.1.2: •

Find $\lim_{x \rightarrow -\infty} \frac{x^5 - 14x^4 + x}{x^2 + x}$

Dividing by the highest power in the denominator (x^2), we get

$$\lim_{x \rightarrow -\infty} \frac{x^3 - 14x^2 + \frac{1}{x}}{1 + \frac{1}{x}}\tag{5}$$

Now the $1/x$ terms go to 0. But $x^3 \rightarrow -\infty$. Since x^3 is the highest power left over in the numerator, it determines what happens. So

$$\lim_{x \rightarrow -\infty} \frac{x^5 - 14x^4 + x}{x^2 + x} = -\infty\tag{6}$$

0.2 Fractions of Polynomials**Example 0.2.1:** •

Find $\lim_{x \rightarrow 4} \frac{x^2 - x - 12}{x - 4}$

The denominator is already factored. Factoring the numerator we have

$$\lim_{x \rightarrow 4} \frac{x^2 - x - 12}{x - 4} = \lim_{x \rightarrow 4} \frac{(x - 4)(x + 3)}{x - 4} \quad (7)$$

Then cancelling $x - 4$, we're left with

$$\lim_{x \rightarrow 4} x + 3 = 4 + 3 = 7 \quad (8)$$

Example 0.2.2: •

Find $\lim_{x \rightarrow -3} \frac{x^2 + 5x + 6}{x^2 - 9}$

Here we need to factor both the numerator and denominator. We get

$$\lim_{x \rightarrow -3} \frac{x^2 + 5x + 6}{x^2 - 9} = \lim_{x \rightarrow -3} \frac{(x + 2)(x + 3)}{(x - 3)(x + 3)} \quad (9)$$

Cancelling $x + 3$, we have

$$\lim_{x \rightarrow -3} \frac{(x + 2)}{(x - 3)} = \frac{-3 + 2}{-3 - 3} = \frac{-1}{-6} = 1/6 \quad (10)$$

0.3 $\sqrt{x + \dots} - n$

Example 0.3.1: •

Find $\lim_{x \rightarrow 4} \frac{x^2 - 4}{\sqrt{x} - 2}$

$$\lim_{x \rightarrow 4} \frac{x^2 - 16}{\sqrt{x} - 2} \left(\frac{\sqrt{x} + 2}{\sqrt{x} + 2} \right) = \lim_{x \rightarrow 4} \frac{(x^2 - 16)(\sqrt{x} + 2)}{x - 4} \quad (11)$$

Now we can factor the numerator (because we have one polynomial divided by another), to get

$$\begin{aligned} \lim_{x \rightarrow 4} \frac{(x - 4)(x + 4)(\sqrt{x} + 2)}{x - 4} &= \lim_{x \rightarrow 4} (x + 4)(\sqrt{x} + 2) \\ &= (4 + 4)(\sqrt{4} + 2) \\ &= 8(2 + 2) \\ &= 32 \end{aligned} \quad (12)$$

Example 0.3.2: •

Find $\lim_{x \rightarrow 5} \frac{x-5}{2-\sqrt{x-1}}$

Here the conjugate is $2+\sqrt{x-1}$. Multiplying by it on the top and bottom we have

$$\lim_{x \rightarrow 5} \frac{(x-5)(2+\sqrt{x-1})}{(2-\sqrt{x-1})(2+\sqrt{x-1})} = \lim_{x \rightarrow 5} \frac{(x-5)(2+\sqrt{x-1})}{4-(x-1)} \quad (13)$$

This is

$$\lim_{x \rightarrow 5} \frac{(x-5)(2+\sqrt{x-1})}{5-x} = \lim_{x \rightarrow 5} \frac{(x-5)(2+\sqrt{x-1})}{-(x-5)} \quad (14)$$

Now we cancel the $x-5$ to get

$$\lim_{x \rightarrow 5} -(2+\sqrt{x-1}) = -(2+\sqrt{5-1}) = -(2+\sqrt{4}) = -(2+2) = -4 \quad (15)$$

0.4 $\frac{\sin nx}{x}$

This is a type of limit you just need to memorize:

$$\lim_{x \rightarrow 0} \frac{\sin nx}{x} = n \quad (16)$$

Example 0.4.1: •

$$\lim_{x \rightarrow 0} \frac{\sin 7x}{x} = 7 \quad (17)$$

Example 0.4.2: •

$$\lim_{x \rightarrow 0} \frac{\sin -5x}{x} = -5 \quad (18)$$

Example 0.4.3: •

$$\lim_{x \rightarrow 0} \frac{x}{\sin \pi x} = \lim_{x \rightarrow 0} \frac{1}{\left(\frac{\sin \pi x}{x}\right)} = \frac{1}{\pi} \quad (19)$$

0.5. $\frac{\sin}{\sin}$

5

0.5 $\frac{\sin}{\sin}$

Example 0.5.1: •

Find $\lim_{x \rightarrow 0} \frac{\sin x}{\sin 10x}$

$$\begin{aligned} \lim_{x \rightarrow 0} \frac{\sin x}{\sin 10x} &= \lim_{x \rightarrow 0} \frac{\sin x}{\sin 10x} \left(\frac{x}{x}\right) \\ &= \lim_{x \rightarrow 0} \frac{\sin x}{x} \frac{x}{\sin 10x} \\ &= 1 \left(\frac{1}{10}\right) \\ &= \frac{1}{10} \end{aligned} \tag{20}$$

Example 0.5.2: •

Find $\lim_{x \rightarrow 0} \frac{\sin(-17x)}{\sin \frac{x}{2}}$

$$\begin{aligned} \lim_{x \rightarrow 0} \frac{\sin(-17x)}{\sin \frac{x}{2}} &= \lim_{x \rightarrow 0} \frac{\sin(-17x)}{\sin \frac{x}{2}} \left(\frac{x}{x}\right) \\ &= \lim_{x \rightarrow 0} \frac{\sin(-17x)}{x} \frac{x}{\sin \frac{x}{2}} \\ &= -17 \left(\frac{1}{1/2}\right) \\ &= -17(2) \\ &= -34 \end{aligned} \tag{21}$$

0.6 $\tan x$

Example 0.6.1: •

Find $\lim_{x \rightarrow 0} \frac{\tan 15x}{\sin 8x}$

First we change the tan into sin and cos

$$\lim_{x \rightarrow 0} \frac{\tan 15x}{\sin 8x} = \lim_{x \rightarrow 0} \frac{\sin 15x}{\cos 15x} \left(\frac{1}{\sin 8x} \right) \quad (22)$$

Next since we have sin / sin we multiply by x/x :

$$\lim_{x \rightarrow 0} \frac{\sin 15x}{\cos 15x} \left(\frac{1}{\sin 8x} \right) \left(\frac{x}{x} \right) = \lim_{x \rightarrow 0} \frac{\sin 15x}{x} \left(\frac{x}{\sin 8x} \right) \left(\frac{1}{\cos 15x} \right) \quad (23)$$

Now $\cos(0) = 1$, so

$$\begin{aligned} \lim_{x \rightarrow 0} \frac{\sin 15x}{x} \left(\frac{x}{\sin 8x} \right) \left(\frac{1}{\cos 15x} \right) &= 15 \left(\frac{1}{8} \right) \left(\frac{1}{1} \right) \\ &= \frac{15}{8} \end{aligned} \quad (24)$$

0.7 $1 - \cos$ or $1 - \sin$

Example 0.7.1: •

Find $\lim_{x \rightarrow \pi} \frac{\sin^2 x}{1 - \cos x}$

$$\lim_{x \rightarrow 2\pi} \frac{\sin^2 x}{1 - \cos x} = \lim_{x \rightarrow 2\pi} \frac{\sin^2 x}{1 - \cos x} \left(\frac{1 + \cos x}{1 + \cos x} \right) \quad (25)$$

$$= \lim_{x \rightarrow 2\pi} \frac{(\sin^2 x)(1 + \cos x)}{1 - \cos^2 x} = \lim_{x \rightarrow 2\pi} \frac{(\sin^2 x)(1 + \cos x)}{\sin^2 x} \quad (26)$$

$$= \lim_{x \rightarrow 2\pi} 1 + \cos x = 1 + 1 = 2 \quad (27)$$